\documentclass{article}
\usepackage{graphicx}

\begin{document}

\title{Technical Questions and Answers in Machine Learning}
\author{ONI Olalekan Joseph}

\maketitle

\section{Problem 2}
Determine the first and second derivative with respect to $x$ of: $f(x)= \frac{1}{1 + e^{-x}} $

\subsection{Solution 2}
 First Derivative: \\
 $f(x) = (1 + e^-x)^{-1}$ \\
 Using Chain Rule \\
 $f'(x) = -1(1 + e^{-x})^{-2} \times -1e^{-x}$ \\
 $f'(x) = \frac{e^{-x}}{(1 + e^{-x})^{2}}$ \\ \\
 
\noindent Second Derivative:  \\
 $f'(x) = \frac{e^{-x}}{(1 + e^{-x})^{2}}$ \\
 Using Quotient Rule of Differentiation \\
 $g(x) = e^{-x}$  \qquad  $h(x) = (1 + e^{-x})^{2}$ \\
 $ g'(x) = -e^{x} $ \qquad $h'(x) = -2e^{-x}(1 + e^{-x}) $ \\
 $f''(x) = \frac{h \times g' - g \times h' }{g^2}  $ \\
 $f''(x) = \frac{-e^{-x} \times (1 + e^{-x})^{2} \enspace + \enspace 2e^{-2x} \times (1 + e^{-x})}{e^{-2x}} $\\
 $f''(x) = \frac{e^{-2x} - 1}{e^{-x}} $

\end{document}